move check_{un,bin}op and correctness results to Operators and ObcToClight.Interface

src/Lustre/Denot/CheckOp.v
@@ -2,17 +2,15 @@ From Coq Require Import Datatypes List.
 Import List.ListNotations.
 
 From Velus Require Import Common.
-From Velus Require Import CommonList.
-From Velus Require Import CommonTyping.
 From Velus Require Import Operators.
 From Velus Require Import Clocks.
 From Velus Require Import Lustre.StaticEnv.
-From Velus Require Import Lustre.LSyntax Lustre.LTyping Lustre.LOrdered.
+From Velus Require Import Lustre.LSyntax Lustre.LTyping.
 
-From Velus Require Import Lustre.Denot.Cpo.
-Require Import CommonDS SDfuns Denot OpErr CommonList2 Restr.
+(** * Little static analysis to decide [OpErr.op_correct] *)
 
-(** * Little static analysis to decide [op_correct] *)
+(* we keep it outside of [OpErr], otherwise the extraction of [check_global]
+ * recursively extracts the CPO library (because of functors...) *)
 
 Module Type CHECKOP
        (Import Ids   : IDS)
@@ -20,51 +18,7 @@ Module Type CHECKOP
        (Import OpAux : OPERATORS_AUX Ids Op)
        (Import Cks   : CLOCKS        Ids Op OpAux)
        (Import Senv  : STATICENV     Ids Op OpAux Cks)
-       (Import Syn   : LSYNTAX       Ids Op OpAux Cks Senv)
-       (Import Typ   : LTYPING       Ids Op OpAux Cks Senv Syn)
-       (Import Restr : LRESTR        Ids Op OpAux Cks Senv Syn)
-       (Import Lord  : LORDERED      Ids Op OpAux Cks Senv Syn)
-       (Import Den   : LDENOT        Ids Op OpAux Cks Senv Syn Lord)
-       (Import OpErr : OP_ERR        Ids Op OpAux Cks Senv Syn Lord Den).
-
-
-(** All check_* functions return a boolean value:
- * - true -> cannot fail
- * - false -> we don't know
- *)
-
-(** Legal unary operators *)
-Parameter check_unop : unop -> type -> bool.
-Conjecture check_unop_correct :
-  forall op ty,
-    check_unop op ty = true ->
-    forall v, wt_value v ty ->
-         sem_unop op v ty <> None.
-
-
-(** There is two cases for binary operators :
- * - we know the value of the right member because it is constant;
- * - we don't know it, so we only authorize operators that never fails
- *)
-
-(* first case *)
-Parameter check_binop_val : binop -> type -> value -> type -> bool.
-Conjecture check_binop_val_correct :
-  forall op ty1 v2 ty2,
-    check_binop_val op ty1 v2 ty2 = true ->
-    forall v1, wt_value v1 ty1 ->
-          wt_value v2 ty2 ->
-          sem_binop op v1 ty1 v2 ty2 <> None.
-
-(* second case *)
-Parameter check_binop_any : binop -> type -> type -> bool.
-Conjecture check_binop_any_correct :
-  forall op ty1 ty2,
-    check_binop_any op ty1 ty2 = true ->
-    forall v1 v2, wt_value v1 ty1 ->
-             wt_value v2 ty2 ->
-             sem_binop op v1 ty1 v2 ty2 <> None.
-
+       (Import Syn   : LSYNTAX       Ids Op OpAux Cks Senv).
 
 (* true -> cannot fail
  * false -> we don't know *)
@@ -76,22 +30,22 @@ Fixpoint check_exp (e : exp) : bool :=
   | Elast _ _ => true (* restr *)
   | Eunop op e ann =>
       match typeof e with
-      | [ty] => check_unop op ty && check_exp e
+      | [ty] => check_unop op None ty && check_exp e
       | _ => true
       end
-  | Ebinop op e1 (Econst c) ann => (* TODO: Enum aussi ? *)
+  | Ebinop op e1 (Econst c) ann =>
       let ty2 := Tprimitive (ctype_cconst c) in
       match typeof e1 with
       | [ty1] => check_exp e1
                 (* soit on arrive à décider avec la valeur c,
                    soit on vérifie pour toute valeur de type ty2 *)
-                && (check_binop_val op ty1 (Vscalar (sem_cconst c)) ty2
-                    || check_binop_any op ty1 ty2)
+                && (check_binop op None ty1 (Some (Vscalar (sem_cconst c))) ty2
+                    || check_binop op None ty1 None ty2)
       | _ => true
       end
   | Ebinop op e1 e2 ann =>
       match typeof e1, typeof e2 with
-      | [ty1], [ty2] => check_binop_any op ty1 ty2 && check_exp e1 && check_exp e2
+      | [ty1], [ty2] => check_binop op None ty1 None ty2 && check_exp e1 && check_exp e2
       | _,_ => true
       end
   | Eextcall _ _ _ => true (* restr *)
@@ -116,127 +70,12 @@ Definition check_top_block b :=
   | _ => false
   end.
 
-Definition check_node (n : node) :=
+Definition check_node {PSyn Prefs} (n : @node PSyn Prefs) :=
   check_top_block (n_block n).
 
-Definition check_global (G : global) := forallb check_node (nodes G).
+Definition check_global {PSyn Prefs} (G : @global PSyn Prefs) :=
+  forallb check_node (nodes G).
 
-
-(** ** Correction of the procedure *)
-
-Theorem check_exp_ok :
-  forall Γ G ins envG envI bs env,
-  forall e, restr_exp e ->
-       wt_exp G Γ e ->
-       check_exp e = true ->
-       op_correct_exp G ins envG envI bs env e.
-Proof.
-  intros *.
-  induction e using exp_ind2; simpl; intros Hr Hwt Hchk; inv Hr; inv Hwt.
-  - (* Econst *)
-    constructor.
-  - (* Eenum *)
-    constructor.
-  - (* Evar *)
-    constructor.
-  - (* Eunop *)
-    destruct (typeof e) as [|? []] eqn:Hty; try congruence.
-    apply andb_prop in Hchk as [F1 F2].
-    constructor; auto.
-    intros ty' Hty'.
-    rewrite Hty' in Hty; inv Hty.
-    (* c'est très très simple *)
-    apply nprod_forall_Forall, Forall_forall.
-    intros s Hin.
-    apply DSForall_all; intros [| v |]; auto.
-    intro Wtv.
-    now apply check_unop_correct.
-  - (* Ebinop *)
-    take (typeof e1 = _) and rewrite it in Hchk.
-    take (typeof e2 = _) and rewrite it in Hchk.
-    constructor.
-    (* récurrence pour e1, e2 *)
-    1,2: cases; repeat rewrite Bool.andb_true_iff in *; tauto.
-    intros ty1' ty2' Hty1' Hty2' ss1 ss2.
-    rewrite Hty1' in *; take ([_] = [_]) and inv it.
-    rewrite Hty2' in *; take ([_] = [_]) and inv it.
-    (* cas sur la tête de e2 *)
-    cases; inv Hty2'; repeat rewrite Bool.andb_true_iff, ?Bool.orb_true_iff in *.
-    (* membre droit constant *)
-    { subst ss2; rewrite denot_exp_eq.
-      simpl.
-      unfold sconst, DSForall_2pres.
-      rewrite ID_simpl, Id_simpl, MAP_map, zip_map.
-      eapply DSForall_zip with (P := fun _ => True) (Q := fun _ => True); auto using DSForall_all.
-      intros [] [] _ _; auto.
-      intros Wt1 Wt2.
-      destruct Hchk as [? []].
-      - apply check_binop_val_correct; auto.
-      - apply check_binop_any_correct; auto. }
-    (* autres cas *)
-    all: apply DSForall_all.
-    all: intros [[|v1|] [|v2|]]; auto; intros Wt1 Wt2.
-    all: apply check_binop_any_correct; auto; tauto.
-  - (* Efby *)
-    apply andb_prop in Hchk as [F1 F2].
-    apply forallb_Forall in F1, F2.
-    constructor; simpl_Forall; auto.
-  - (* Ewhen *)
-    apply forallb_Forall in Hchk.
-    constructor; simpl_Forall; auto.
-  - (* Emerge *)
-    apply forallb_Forall in Hchk.
-    constructor; simpl_Forall.
-    eapply forallb_Forall, Forall_forall in Hchk; eauto.
-  - (* Ecase default *)
-    apply andb_prop in Hchk as [F1 F2].
-    apply forallb_Forall in F2.
-    constructor; simpl_Forall; auto.
-    eapply forallb_Forall, Forall_forall in F2; eauto.
-  - (* Ecase *)
-    apply andb_prop in Hchk as [F1 F3].
-    apply andb_prop in F1 as [F1 F2].
-    apply forallb_Forall in F2,F3.
-    constructor; simpl_Forall; auto.
-    eapply forallb_Forall, Forall_forall in F2; eauto.
-  - (* Eapp *)
-    apply andb_prop in Hchk as [F1 F2].
-    apply forallb_Forall in F1, F2.
-    constructor; simpl_Forall; auto.
-Qed.
-
-Lemma check_block_ok :
-  forall Γ G ins envG envI bs env,
-  forall b, restr_block b ->
-       wt_block G Γ b ->
-       check_block b = true ->
-       op_correct_block G ins envG envI bs env b.
-Proof.
-  destruct b; simpl; intros * Hr Hwt Hc; try tauto.
-  destruct e.
-  eapply forallb_Forall in Hc.
-  inv Hr; inv Hwt.
-  simpl_Forall; eauto using check_exp_ok.
-Qed.
-
-Lemma check_node_ok :
-  forall G ins envG envI bs env,
-  forall (n : node),
-    restr_node n ->
-    wt_node G n ->
-    check_node n = true ->
-    op_correct G ins envG envI bs env n.
-Proof.
-  unfold check_node, check_top_block, op_correct.
-  intros * Hr Hwt Hc.
-  inv Hr; inv Hwt.
-  cases.
-  take (restr_top_block _) and inv it.
-  take (wt_block _ _ _) and inv it.
-  take (wt_scope _ _ _ _) and inv it.
-  apply forallb_Forall in Hc.
-  simpl_Forall; eauto using check_block_ok.
-Qed.
 
 End CHECKOP.
 
@@ -247,11 +86,6 @@ Module CheckOpFun
   (Cks   : CLOCKS        Ids Op OpAux)
   (Senv  : STATICENV     Ids Op OpAux Cks)
   (Syn   : LSYNTAX       Ids Op OpAux Cks Senv)
-  (Typ   : LTYPING       Ids Op OpAux Cks Senv Syn)
-  (Restr : LRESTR        Ids Op OpAux Cks Senv Syn)
-  (Lord  : LORDERED      Ids Op OpAux Cks Senv Syn)
-  (Den   : LDENOT        Ids Op OpAux Cks Senv Syn Lord)
-  (OpErr : OP_ERR        Ids Op OpAux Cks Senv Syn Lord Den)
-<: CHECKOP Ids Op OpAux Cks Senv Syn Typ Restr Lord Den OpErr.
-  Include CHECKOP Ids Op OpAux Cks Senv Syn Typ Restr Lord Den OpErr.
+<: CHECKOP Ids Op OpAux Cks Senv Syn.
+  Include CHECKOP Ids Op OpAux Cks Senv Syn.
 End CheckOpFun.
